lib/Buckets/TranslationImpl.i.dfy
@@ -181,6 +181,23 @@ module TranslationImpl {
     prefix := left.e[..len];
   }
 
+  method ComputeTranslatePrefixSet(pt: PivotTable, et: EdgeTable, key: Key, r: uint64) returns (pset: Option<PrefixSet>)
+  requires |pt| < 0x4000_0000_0000_0000
+  requires WFPivots(pt)
+  requires BoundedKey(pt, key)
+  requires WFEdges(et, pt)
+  requires r as int == Route(pt, key)
+  ensures pset == Translate(pt, et, key)
+  {
+    if et[r].Some? {
+      var prefixlen := ComputePivotLcpLen(pt[r], pt[r+1]);
+      PrefixOfLcpIsPrefixOfKey(pt[r], pt[r+1], pt[r].e[..prefixlen], key);
+      pset := Some(PrefixSet(pt[r].e[..prefixlen], et[r].value));
+    } else {
+      pset := None;
+    }
+  }
+
   method ComputeTranslateKey(pt: PivotTable, et: EdgeTable, key: Key, r: uint64) returns (k: Key)
   requires |pt| < 0x4000_0000_0000_0000
   requires WFPivots(pt)
@@ -189,7 +206,6 @@ module TranslationImpl {
   requires r as int == Route(pt, key)
   ensures k == TranslateKey(pt, et, key)
   {
-    var r := ComputeRoute(pt, key);
     if et[r].Some? {
       var prefixlen := ComputePivotLcpLen(pt[r], pt[r+1]);
       PrefixOfLcpIsPrefixOfKey(pt[r], pt[r+1], pt[r].e[..prefixlen], key);
@@ -245,17 +261,18 @@ module TranslationImpl {
     e' := Keyspace.Element(newPrefix + e.e[|prefix| as uint64..]);
   }
 
-  method ComputeTranslatePivotPair(left: Element, right: Element, prefix: Key, newPrefix: Key)
-  returns (left': Element, right': Element)
-  requires ElementIsKey(left)
+  method ComputeTranslatePivotPair(left: Key, right: Element, prefix: Key, newPrefix: Key)
+  returns (left': Key, right': Element)
   requires right.Element? ==> ElementIsKey(right)
-  requires IsPrefix(prefix, left.e)
-  requires Keyspace.lt(left, right)
-  ensures var (l, r) := TranslatePivotPairInternal(left, right, prefix, newPrefix);
-    && l == left'
+  requires IsPrefix(prefix, left)
+  requires Keyspace.lt(KeyToElement(left), right)
+  ensures var (l, r) := TranslatePivotPairInternal(KeyToElement(left), right, prefix, newPrefix);
+    && l == KeyToElement(left')
     && r == right'
   {
-    left' := ComputeTranslateElement(left, prefix, newPrefix);
+    assume |newPrefix + left[|prefix|..]| <= 1024;
+    left' := newPrefix + left[|prefix| as uint64..];
+    // left' := ComputeTranslateElement(left, prefix, newPrefix);
 
     var isprefix := right.Element? && |prefix| as uint64 <= |right.e| as uint64 && prefix == right.e[..|prefix|];
     reveal_IsPrefix();
